library/init/meta/congruence_tactics.lean
@@ -12,7 +12,6 @@ meta constant cc_state.mk           : cc_state
 /- Create a congruence closure state object using the hypotheses in the current goal. -/
 meta constant cc_state.mk_using_hs  : tactic cc_state
 meta constant cc_state.next         : cc_state → expr → expr
-meta constant cc_state.inconsistent : cc_state → bool
 meta constant cc_state.roots_core   : cc_state → bool → list expr
 meta constant cc_state.root         : cc_state → expr → expr
 meta constant cc_state.mt           : cc_state → expr → nat
@@ -24,7 +23,9 @@ meta constant cc_state.add          : cc_state → expr → tactic cc_state
 meta constant cc_state.is_eqv       : cc_state → expr → expr → tactic bool
 meta constant cc_state.is_not_eqv   : cc_state → expr → expr → tactic bool
 meta constant cc_state.eqv_proof    : cc_state → expr → expr → tactic expr
-
+meta constant cc_state.inconsistent : cc_state → bool
+/- If the given state is inconsistent, return a proof for false. Otherwise fail. -/
+meta constant cc_state.false_proof  : cc_state → tactic expr
 namespace cc_state
 
 meta def roots (s : cc_state) : list expr :=
@@ -48,3 +49,18 @@ meta def eqc_size (s : cc_state) (e : expr) : nat :=
 (s^.eqc_of e)^.length
 
 end cc_state
+
+open tactic
+meta def tactic.cc : tactic unit :=
+do intros, s ← cc_state.mk_using_hs, t ← target, s ← s^.internalize t tt,
+   if s^.inconsistent then do {
+     pr ← s^.false_proof,
+     mk_app `false.elim [t, pr] >>= exact}
+   else do {
+     tr ← return $ expr.const `true [],
+     b ← s^.is_eqv t tr,
+     if b then do {
+       pr ← s^.eqv_proof t tr,
+       mk_app `of_eq_true [pr] >>= exact}
+     else fail "cc tactic failed"
+   }
